added heterogeneous event refinement and reproved meta theory up to iter rule

theories/HeterogeneousEventRelations.v
@@ -32,6 +32,58 @@ Definition relationEAnsH (E1 E2 : Type -> Type) : Type := forall A B, E1 A -> A 
 
 Variant sum_relAns {E1 E2 F1 F2} (REE : relationEAnsH E1 E2) (REF : relationEAnsH F1 F2) : 
   forall A B, (E1 +' F1) A -> A -> (E2 +' F2) B -> B -> Prop :=
-| sum_relEAns_inl A B (e1 : E1 A) (e2 : E2 B) a b : REE A B e1 a e2 b -> sum_relAns REE REF A B (inl1 e1) a (inl1 e2) b
-| sum_relEAns_inr A B (f1 : F1 A) (f2 : F2 B) a b : REF A B f1 a f2 b -> sum_relAns REE REF A B (inr1 f1) a (inr1 f2) b
+| sum_relAns_inl A B (e1 : E1 A) (e2 : E2 B) a b : REE A B e1 a e2 b -> sum_relAns REE REF A B (inl1 e1) a (inl1 e2) b
+| sum_relAns_inr A B (f1 : F1 A) (f2 : F2 B) a b : REF A B f1 a f2 b -> sum_relAns REE REF A B (inr1 f1) a (inr1 f2) b
 .
+
+Definition relationEAns (E1 E2 : Type -> Type) : Type := forall A B, E1 A -> E2 B -> A -> B -> Prop.
+
+
+Variant sum_relEAns {E1 E2 F1 F2} (REE : relationEAns E1 E2) (REF : relationEAns F1 F2) : 
+  forall A B, (E1 +' F1) A -> (E2 +' F2) B -> A -> B -> Prop :=
+| sum_relEAns_inl A B (e1 : E1 A) (e2 : E2 B) a b : REE A B e1 e2 a b -> sum_relEAns REE REF A B (inl1 e1) (inl1 e2) a b
+| sum_relEAns_inr A B (f1 : F1 A) (f2 : F2 B) a b : REF A B f1 f2 a b -> sum_relEAns REE REF A B (inr1 f1) (inr1 f2) a b
+.
+
+(* This may need to be defined in dependent on two relationEH's?*)
+(*
+Variant rcomposeEAns' {E1 E2 E3 : Type -> Type}
+           (RE12 : relationEAns E1 E2) (RE23 : relationEAns E2 E3): 
+  forall A C, E1 A -> E3 C -> A -> C -> Prop :=
+  | rcomposeEAns_intro (A B C : Type) 
+                       (*maybe I should somehow universally quantify this*)
+                       (e1 : E1 A) (e2 : E2 B) (e3 : E3 C)
+                       a b c :
+    RE12 A B e1 e2 a b -> RE23 B C e2 e3 b c ->
+    rcomposeEAns RE12 RE23 A C e1 e3 a c.
+*)
+
+
+(* this means that if I find an e2, there must be a b that we can link
+   the two with,
+   the problem is what if the post condition is empty I should think of 
+   a new case for this possibility
+ *)
+Variant rcomposeEAns {E1 E2 E3 : Type -> Type}
+           (RE12 : relationEAns E1 E2) (RE23 : relationEAns E2 E3)
+           (RE : forall A B C, E1 A -> E2 B -> E3 C -> Prop)
+  : 
+  forall A C, E1 A -> E3 C -> A -> C -> Prop :=
+  | rcomposeEAns_intro (A C : Type) 
+                       (e1 : E1 A) (e3 : E3 C)
+                       a c :
+    (forall B (e2 : E2 B), 
+      RE A B C e1 e2 e3 -> exists b, RE12 A B e1 e2 a b /\ RE23 B C e2 e3 b c) ->
+    rcomposeEAns RE12 RE23 RE A C e1 e3 a c.
+
+(*this is stronger than I need*)
+(* I see 2 ways to do it, either it is reflexive wrt RE
+   or *)
+Class ReflexiveEAns {E : Type -> Type} (REA : relationEAns E E) :  Prop :=
+  reflexiveEAns : forall A (e : E A) (a b : A), 
+      REA A A e e a b -> a = b.
+
+Class SymmetricEAns {E : Type -> Type} (REA : relationEAns E E) : Prop :=
+  symmetricEAns : forall A B (e1 : E A) (e2 : E B) a b,
+      REA A B e1 e2 a b -> REA B A e2 e1 b a.
+
