theories/Refinement.v
@@ -170,25 +170,22 @@ Proof.
 Qed.
 (* Print Assumptions not_Proper_eutt_satisfies_impl. *)
 
-Instance Proper_eutt_satisfies {E R1 R2} RR :
-  Proper (eutt eq ==> eutt eq ==> iff) (@satisfies E R1 R2 RR).
-Proof.
-  repeat intro.
-Abort.
-
-
+Section Refines.
 (***
  *** Refinement of itree specs
  ***)
 
+Context {E1 E2 : Type -> Type} {R1 R2 : Type}.
+Context (RE : relationEH E1 E2) (REAns : relationEAns E1 E2) (RR : R1 -> R2 -> Prop).
+
 (* One itree_spec refines another iff, after turning finitely many quantifier
 events to actual quantifiers, they have the same constructor with continuations
 such that the first continuation coinductively refines the second *)
-Inductive refinesF {E1 E2 R1 R2} (RE : forall (A B : Type), E1 A -> E2 B -> Prop ) (RR : R1 -> R2 -> Prop) (F : itree_spec E1 R1 -> itree_spec E2 R2 -> Prop) : 
+Inductive refinesF  (F : itree_spec E1 R1 -> itree_spec E2 R2 -> Prop) : 
   itree_spec' E1 R1 -> itree_spec' E2 R2 -> Prop :=
-  | refines_Ret r1 r2 : RR r1 r2 -> refinesF RE RR F (RetF r1) (RetF r2)
+  | refines_Ret r1 r2 : RR r1 r2 -> refinesF F (RetF r1) (RetF r2)
   | refines_TauLR phi1 phi2 :
-      F phi1 phi2 -> refinesF RE RR F (TauF phi1) (TauF phi2)
+      F phi1 phi2 -> refinesF F (TauF phi1) (TauF phi2)
 (*
   | refines_TauL phi ophi :
       refinesF F (observe phi) ophi -> refinesF F (TauF phi) ophi
@@ -196,44 +193,46 @@ Inductive refinesF {E1 E2 R1 R2} (RE : forall (A B : Type), E1 A -> E2 B -> Prop
       refinesF F ophi (observe phi) -> refinesF F ophi (TauF phi)
 *)
   | refines_VisLR A B e1 e2 kphi1 kphi2 :
-      RE A B e1 e2 -> (* need some notion of RAns, possibly stuffed into *)
-      (forall a b, F (kphi1 a) (kphi2 b) ) ->
-      refinesF RE RR F (VisF (Spec_vis e1) kphi1) (VisF (Spec_vis e2) kphi2)
-  | refines_VisLRForall A B kphi1 kphi2 :
-      (forall (a : A) (b : B), F (kphi1 a) (kphi2 b) ) ->
-      refinesF RE RR F (VisF Spec_forall kphi1) (VisF Spec_forall kphi2)
-  | refines_VisLRExists A B kphi1 kphi2 :
-      (forall (a : A) (b : B), F (kphi1 a) (kphi2 b) ) ->
-      refinesF RE RR F (VisF Spec_exists kphi1) (VisF Spec_exists kphi2)
+      RE A B e1 e2 ->
+      (forall a b, REAns A B e1 e2 a b -> F (kphi1 a) (kphi2 b) ) ->
+      refinesF F (VisF (Spec_vis e1) kphi1) (VisF (Spec_vis e2) kphi2)
+
+  (*removing these rules may help with simplicity*)
+  | refines_VisLRForall A kphi1 kphi2 :
+      (forall (a : A), F (kphi1 a) (kphi2 a) ) ->
+      refinesF F (VisF Spec_forall kphi1) (VisF Spec_forall kphi2)
+  | refines_VisLRExists A kphi1 kphi2 :
+      (forall (a : A), F (kphi1 a) (kphi2 a) ) ->
+      refinesF F (VisF Spec_exists kphi1) (VisF Spec_exists kphi2)
   | refines_forallR A kphi phi :
-      (forall a : A, refinesF RE RR F phi (observe (kphi a))) ->
-      refinesF RE RR F phi (VisF Spec_forall kphi)
+      (forall a : A, refinesF F phi (observe (kphi a))) ->
+      refinesF F phi (VisF Spec_forall kphi)
   | refines_forallL A kphi phi (a : A) :
-      (refinesF RE RR F (observe (kphi a)) phi) ->
-      refinesF RE RR F (VisF Spec_forall kphi) phi
+      (refinesF F (observe (kphi a)) phi) ->
+      refinesF F (VisF Spec_forall kphi) phi
   | refines_existsR A kphi phi (a : A) :
-      (refinesF RE RR F phi (observe (kphi a))) ->
-      refinesF RE RR F phi (VisF Spec_exists kphi)
+      (refinesF F phi (observe (kphi a))) ->
+      refinesF F phi (VisF Spec_exists kphi)
   | refines_existsL A kphi phi :
-      (forall a : A, refinesF RE RR F (observe (kphi a)) phi) ->
-      refinesF RE RR F (VisF Spec_exists kphi) phi
+      (forall a : A, refinesF F (observe (kphi a)) phi) ->
+      refinesF F (VisF Spec_exists kphi) phi
 .
 Hint Constructors refinesF.
-Definition refines_ {E1 E2 R1 R2} RE RR F (t1 : itree_spec E1 R1) (t2 : itree_spec E2 R2) : Prop :=
-  refinesF RE RR F (observe t1) (observe t2).
+Definition refines_  F (t1 : itree_spec E1 R1) (t2 : itree_spec E2 R2) : Prop :=
+  refinesF F (observe t1) (observe t2).
 
-Lemma monotone_refinesF {E1 E2 R1 R2} RE RR ot1 ot2 sim sim' 
+Lemma monotone_refinesF ot1 ot2 sim sim' 
   (LE : sim <2= sim' )
-  (IN : @refinesF E1 E2 R1 R2 RE RR sim ot1 ot2) : 
-  refinesF RE RR sim' ot1 ot2.
+  (IN : refinesF sim ot1 ot2) : 
+  refinesF sim' ot1 ot2.
 Proof.
   induction IN; eauto.
 Qed.
 
-Lemma monotone_refines_ {E1 E2 R1 R2} RE RR : monotone2 (@refines_ E1 E2 R1 R2 RE RR).
+Lemma monotone_refines_  : monotone2 refines_.
 Proof. red. intros. eapply monotone_refinesF; eauto. Qed.
 
-Hint Resolve monotone_refines_ : paco.
+
 (*
 Instance Proper_upaco2_refines_ {E R} :
   Proper ((eq ==> eq ==> impl) ==> eq ==> eq ==> impl) (upaco2 (@refines_ E R)).
@@ -266,26 +265,26 @@ Proof.
 Qed.
 *)
 
-Definition refines {E1 E2 R1 R2} RE RR : itree_spec E1 R1 -> itree_spec E2 R2 -> Prop :=
-  paco2 (refines_ RE RR) bot2.
-(*
-Instance Proper_observing_eq_refines {E R} :
-  Proper (observing eq ==> observing eq ==> impl) (@refines E R).
-Proof.
-  unfold Proper, respectful, impl.
-  intros t1 t2 e12 t3 t4 e34 r13. destruct e12 as [e12]. destruct e34 as [e34].
-  pfold. punfold r13. unfold refines_ in * |- *.
-  rewrite e12 in r13. rewrite e34 in r13.
-  assumption.
-Qed.
-*)
+Definition refines : itree_spec E1 R1 -> itree_spec E2 R2 -> Prop :=
+  paco2 refines_ bot2.
+
+End Refines.
+
+#[global] Hint Resolve monotone_refines_ : paco.
+
+Hint Constructors refinesF.
+
 (* need a little library of heterogeneous event relations to express theorems  *)
 
 (* Reflexivity of refinement *)
-Instance Reflexive_refines {E R} RE RR : ReflexiveE RE -> Reflexive RR -> Reflexive (@refines E E R R RE RR).
+Instance Reflexive_refines {E R} RE REAns RR : 
+  ReflexiveE RE -> ReflexiveEAns REAns -> Reflexive RR -> Reflexive (@refines E E R R RE REAns RR).
 Proof.
-  red. pcofix CIH. intros HRR HRE t. pfold. red.
+  red. pcofix CIH. intros HRR HRE HREAns t. pfold. red.
   destruct (observe t); try destruct e; econstructor; eauto.
+  intros. right. apply HRE in H. subst. eauto.
+Qed.
+
   (* this exposes a flaw in current definition, could fix by adding restrictions to return values of events like I do in rutt, in the mrec rule it seems like that would be neccesary
 
   when I make a two related recursive calls, I feel like I need to know that the call events return related
@@ -307,34 +306,36 @@ Proof.
   
   although maybe it is simpler to define refines as hrefines eq eq
 *)
-Qed.
 
-Lemma refines_Vis_forallR : forall (E : Type -> Type) (R1 R2 A : Type) RR (t : itree_spec E R1) (k : A -> itree_spec E R2),
-         refines RR t (Vis Spec_forall k) ->
-         forall a : A, refines RR t (k a).
+Lemma refines_Vis_forallR : forall (E1 E2 : Type -> Type) (R1 R2 A : Type) RE REAns RR 
+                              (t : itree_spec E1 R1) (k : A -> itree_spec E2 R2),
+         refines RE REAns RR t (Vis Spec_forall k) ->
+         forall a : A, refines RE REAns RR t (k a).
 Proof.
-  intros E R1 R2 A RR. pcofix CIH. intros t k Href a.
+  intros E1 E2 R1 R2 A RE RAns RR. pcofix CIH. intros t k Href a.
   pfold. revert a. red. punfold Href. red in Href.
   cbn in *. remember (observe t) as ot. clear Heqot.
   remember (VisF Spec_forall k) as x.
   hinduction Href before r; intros; inv Heqx; inj_existT; subst; pclearbot.
   - econstructor. Unshelve. 2 : apply a. specialize (H a).
-    assert (paco2 (refines_ RR) r (kphi1 a) (k a)). eapply paco2_mon; intros; try contradiction; eauto.
-    inv PR. punfold H0.
-  - clear H0. assert (refines RR (go phi) (k a) ).
+    assert (paco2 (refines_ RE RAns RR) r (kphi1 a) (k a)).
+    eapply paco2_mon; intros; eauto; try contradiction.
+    pstep_reverse.
+  - clear H0. assert (refines RE RAns RR (go phi) (k a) ).
     { pstep. apply H. }
-    enough (paco2 (refines_ RR) r (go phi) (k a) ).
+    enough (paco2 (refines_ RE RAns RR) r (go phi) (k a) ).
     { punfold H1. }
     eapply paco2_mon; eauto. intros; contradiction.
   - econstructor. Unshelve. 2 : apply a. eapply IHHref; eauto.
   - econstructor. intros. eapply H0; eauto.
 Qed.
 
-Lemma refines_Vis_existsL : forall (E : Type -> Type) (R1 R2 A : Type) RR (t : itree_spec E R1) (k : A -> itree_spec E R2),
-         refines RR (Vis Spec_exists k) t ->
-         forall a : A, refines RR (k a) t.
+Lemma refines_Vis_existsL : forall (E1 E2 : Type -> Type) (R1 R2 A : Type) RE REAns RR 
+                              (t : itree_spec E1 R1) (k : A -> itree_spec E2 R2),
+         refines RE REAns RR (Vis Spec_exists k) t ->
+         forall a : A, refines RE REAns RR (k a) t.
 Proof.
-  intros E R1 R2 A RR. intros t k Href.
+  intros E1 E2 R1 R2 A RE REAns RR. intros t k Href.
   intros. pfold. red. punfold Href. red in Href.
   remember (observe t) as ot. clear Heqot. cbn in *.
   remember (VisF Spec_exists k) as x. 
@@ -348,69 +349,63 @@ Qed.
 
 
 (* A version of refinesF specialized to a forall on the left *)
-Inductive forallRefinesF {E R1 R2} (RR : R1 -> R2 -> Prop) (F : itree_spec E R1 -> itree_spec E R2 -> Prop)
-          {A} (kphi1: A -> itree_spec E R1)
-  : itree_spec' E R2 -> Prop :=
+Inductive forallRefinesF {E1 E2 R1 R2} RE RAns (RR : R1 -> R2 -> Prop) (F : itree_spec E1 R1 -> itree_spec E2 R2 -> Prop)
+          {A} (kphi1: A -> itree_spec E1 R1)
+  : itree_spec' E2 R2 -> Prop :=
   | forallRefines_VisLR kphi2 :
       (forall a : A, F (kphi1 a) (kphi2 a)) ->
-      forallRefinesF RR F kphi1 (VisF Spec_forall kphi2)
+      forallRefinesF RE RAns RR F kphi1 (VisF Spec_forall kphi2)
   | forallRefines_forallR B kphi2 :
-      (forall b : B, forallRefinesF RR F kphi1 (observe (kphi2 b))) ->
-      forallRefinesF RR F kphi1 (VisF Spec_forall kphi2)
+      (forall b : B, forallRefinesF RE RAns RR F kphi1 (observe (kphi2 b))) ->
+      forallRefinesF RE RAns RR F kphi1 (VisF Spec_forall kphi2)
   | forallRefines_forallL phi (a : A) :
-      refinesF RR F (observe (kphi1 a)) phi ->
-      forallRefinesF RR F kphi1 phi
+      refinesF RE RAns RR F (observe (kphi1 a)) phi ->
+      forallRefinesF RE RAns RR F kphi1 phi
   | forallRefines_existsR B kphi2 (b : B) :
-      (forallRefinesF RR F kphi1 (observe (kphi2 b))) ->
-      forallRefinesF RR F kphi1 (VisF Spec_exists kphi2)
+      (forallRefinesF RE RAns RR F kphi1 (observe (kphi2 b))) ->
+      forallRefinesF RE RAns RR F kphi1 (VisF Spec_exists kphi2)
 .
 
 (* FIXME: should we replace the recursive call to refinesF in the above with
 just a refines? *)
 
-Lemma refinesF_Vis_forallL : forall (E : Type -> Type) (R1 R2 A : Type) RR F
-                                   (t : itree_spec' E R2) (k : A -> itree_spec E R1),
-    refinesF RR F (VisF Spec_forall k) t ->
-    @forallRefinesF E R1 R2 RR F A k t.
+Lemma refinesF_Vis_forallL : forall (E1 E2 : Type -> Type) (R1 R2 A : Type) RE RAns RR F
+                                   (t : itree_spec' E2 R2) (k : A -> itree_spec E1 R1),
+    refinesF RE RAns RR F (VisF Spec_forall k) t ->
+    @forallRefinesF E1 E2 R1 R2 RE RAns RR F A k t.
 Proof.
   intros. remember (VisF Spec_forall k) as t1. induction H.
   - inversion Heqt1.
   - inversion Heqt1.
-  - assert (A0=A); [ inversion Heqt1; reflexivity | ].
-    revert e kphi1 Heqt1 kphi2 H; rewrite H0; intros.
-    assert (kphi1=k); [ inversion Heqt1; inj_existT; assumption | ].
-    rewrite H1 in H.
-    assert (e=Spec_forall); [ inversion Heqt1; inj_existT; assumption | ].
-    rewrite H2.
-    apply forallRefines_VisLR. apply H.
-  - apply forallRefines_forallR. intro b. apply H0. assumption.
-  - assert (A0=A); [ inversion Heqt1; reflexivity | ].
-    revert kphi Heqt1 a H IHrefinesF; rewrite H0; intros.
-    assert (kphi=k); [ inversion Heqt1; inj_existT; assumption | ].
-    rewrite H1 in H.
-    eapply forallRefines_forallL; eassumption.
-  - eapply forallRefines_existsR. apply IHrefinesF. assumption.
+  - inversion Heqt1.
+  - inversion Heqt1. subst. inj_existT. subst.
+    constructor. auto.
+  - inversion Heqt1. 
+  - constructor. auto.
+  - inversion Heqt1. subst. inj_existT; subst. econstructor; eauto.
+  - subst.
+    eapply forallRefines_existsR. eauto.
   - inversion Heqt1.
 Qed.
 
-
+(* not sure what is wrong here *)
 (* A version of refinesF specialized to a Tau on the left *)
-Inductive tauRefinesF {E R1 R2} (RR : R1 -> R2 -> Prop) (F : itree_spec E R1 -> itree_spec E R2 -> Prop)
-          (phi1: itree_spec E R1)
-  : itree_spec' E R2 -> Prop :=
+Inductive tauRefinesF {E1 E2 R1 R2} (RR : R1 -> R2 -> Prop) (F : itree_spec E1 R1 -> itree_spec E2 R2 -> Prop)
+          (phi1: itree_spec E1 R1)
+  : itree_spec' E2 R2 -> Prop :=
   | tauRefines_VisLR phi2 : F phi1 phi2 -> tauRefinesF RR F phi1 (TauF phi2)
   | tauRefines_forallR B kphi2 :
-      (forall b : B, tauRefinesF RR F phi1 (observe (kphi2 b))) ->
-      tauRefinesF RR F phi1 (VisF Spec_forall kphi2)
+      (forall b : B, tauRefinesF  RR F phi1 (observe (kphi2 b))) ->
+      tauRefinesF  RR F phi1 (VisF Spec_forall kphi2)
   | tauRefines_existsR B kphi2 (b : B) :
       tauRefinesF RR F phi1 (observe (kphi2 b)) ->
       tauRefinesF RR F phi1 (VisF Spec_exists kphi2)
 .
 
-Lemma refinesF_Tau : forall (E : Type -> Type) (R1 R2 : Type) RR F
-                            t1 (t2 : itree_spec' E R2),
-    refinesF RR F (TauF t1) t2 ->
-    @tauRefinesF E R1 R2 RR F t1 t2.
+Lemma refinesF_Tau : forall (E1 E2 : Type -> Type) (R1 R2 : Type) RE REAns RR F
+                            t1 (t2 : itree_spec' E2 R2),
+    refinesF RE REAns RR F (TauF t1) t2 ->
+    @tauRefinesF E1 E2 R1 R2 RR F t1 t2.
 Proof.
   intros. remember (TauF t1) as t. induction H; inversion Heqt.
   - rewrite <- H1. constructor. assumption.
@@ -455,9 +450,14 @@ Proof.
 Qed.
 
 (* Transitivity of refinement if the LHS is concrete *)
-Theorem concreteRefinesTrans {E R1 R2 R3} (RR1 : R1 -> R2 -> Prop) (RR2 : R2 -> R3 -> Prop) t1 t2 t3
+Theorem concreteRefinesTrans {E1 E2 E3 R1 R2 R3} RE1 RE2 REAns1 REAns2 
+        (RR1 : R1 -> R2 -> Prop) (RR2 : R2 -> R3 -> Prop) 
+        (t1 : itree_spec E1 R1) (t2 : itree_spec E2 R2) (t3 : itree_spec E3 R3)
          (isc:isConcrete t1) :
-  @refines E _ _ RR1 t1 t2 -> refines RR2 t2 t3 -> refines (rcompose RR1 RR2) t1 t3.
+  refines RE1 REAns1 RR1 t1 t2 -> refines RE2 REAns2 RR2 t2 t3 -> 
+  refines (rcomposeE RE1 RE2) (rcomposeEAns REAns1 REAns2 
+                                  (fun A B C e1 e2 e3 => RE1 A B e1 e2 /\ RE2 B C e2 e3 ) ) 
+          (rcompose RR1 RR2) t1 t3.
 Proof.
   revert t1 t2 t3 isc; pcofix CIH. intros t1 t2 t3 isc Ht12 Ht23.
   pfold. red. punfold Ht12. red in Ht12.
@@ -467,32 +467,45 @@ Proof.
   hinduction Ht12 before r; intros.
   - remember (RetF r2) as x.
     hinduction Ht23 before r; intros; inv Heqx; eauto.
+    constructor. econstructor; eauto.
   - pclearbot. remember (TauF phi2) as x. inversion isc.
     hinduction Ht23 before r; intros; inv Heqx; pclearbot; eauto.
-  - pclearbot. destruct e.
-    + remember (VisF (Spec_vis e) kphi2) as x.
+  - pclearbot. 
+    (* this is where the new reasoning is focused at the moment *)
+    remember (VisF (Spec_vis e2) kphi2) as x.
       hinduction Ht23 before r; intros; inv Heqx; inj_existT; subst; eauto.
-      pclearbot. econstructor. right. eapply CIH; try apply H0; try apply H.
-      eapply (isConcreteVisInv e0). pfold. apply isc.
-    + inversion isc.
-    + inversion isc.
-  - remember (refinesF_Vis_forallL _ _ _ _ _ _ _ _ Ht23) as Ht23'.
-    clear HeqHt23' Ht23. induction Ht23'.
-    * apply refines_forallR. intro a.
+    rename H0 into HRR2. rename H2 into HRR1.
+    constructor. econstructor; eauto. intros.
+    right. 
+    inv H0.
+    subst. inj_existT. subst.
+    specialize (H8 B0 e3).
+    assert (Hb0 :  exists b0 : B0, REAns1 A0 B0 e0 e3 a b0 /\ REAns2 B0 B e3 e2 b0 b).
+    eapply H8; split; eauto.
+    decompose record Hb0. rename x into b0.
+    eapply CIH; eauto.
+    eapply isConcreteVisInv. pstep. eauto.
+    eapply HRR1 in H2; eauto. destruct H2; try contradiction; eauto.
+    eapply HRR2 in H3; destruct H3; try contradiction; eauto.
+  - inv isc.
+  - inv isc.
+  - remember (refinesF_Vis_forallL _ _ _ _ _ _ _ _ _ _ _ Ht23) as Ht23'.
+    clear HeqHt23' Ht23. induction Ht23'; pclearbot.
+    * apply refines_forallR. intro a. pclearbot.
       eapply H0; [ apply CIH | assumption | ]. pstep_reverse.
       destruct (H1 a); [eauto | contradiction].
     * apply refines_forallR. intro b. apply H2.
     * eapply H0; eassumption.
     * eapply refines_existsR. eassumption.
   - inversion isc.
-  - assert (refines RR2 (Vis Spec_exists kphi) (go ot3)); [ pfold; apply Ht23 | ].
+  - assert (refines RE2 REAns2 RR2 (Vis Spec_exists kphi) (go ot3)); [ pfold; apply Ht23 | ].
     apply IHHt12; try assumption.
-    remember (refines_Vis_existsL _ _ _ _ _ (go ot3) kphi H a). clear Heqr0.
+    remember (refines_Vis_existsL _ _ _ _ _ _ _ _ (go ot3) kphi H a). clear Heqr0.
     red in r0. punfold r0.
   - inversion isc.
 Qed.
 
-
+(*
 (* Refinement defines a subset for satisfaction *)
 Theorem refinesSatisfiesSubset {E R1 R2 R3} (RR1 : R1 -> R2 -> Prop) (RR2 : R2 -> R3 -> Prop) 
         (t1 : itree E R1) t2 t3 :
@@ -531,27 +544,27 @@ Proof.
     remember (refines_Vis_existsL _ _ _ _ _ (go ot3) kphi H a). clear Heqr0.
     red in r0. punfold r0.
 Qed.
-
+*)
 Ltac use_simpobs := repeat match goal with
                            | H : RetF _ = observe ?t |- _ => apply simpobs in H 
                            | H : TauF _ = observe ?t |- _ => apply simpobs in H
                            | H : VisF _ _ = observe ?t |- _ => apply simpobs in H
                            end.
 
-Instance eq_itree_refines_Proper1 {E R1 R2 RR r} :  Proper (eq_itree eq ==> eq_itree eq ==> flip impl) 
-                                                           (@refines_ E R1 R2 RR (upaco2 (refines_ RR) r)).
+Instance eq_itree_refines_Proper1 {E1 E2 R1 R2 RE REAns RR r} :  Proper (eq_itree eq ==> eq_itree eq ==> flip impl) 
+                                                           (@refines_ E1 E2 R1 R2 RE REAns RR (upaco2 (refines_ RE REAns RR) r)).
 Admitted. (* needs an axiom to prove this *)
 
-Instance eq_itree_refines_Proper2 {E R1 R2 RR r} :  Proper (eq_itree eq ==> eq_itree eq ==> flip impl) 
-                                                           (paco2 (@refines_ E R1 R2 RR) r).
+Instance eq_itree_refines_Proper2 {E1 E2 R1 R2 RE REAns RR r} :  Proper (eq_itree eq ==> eq_itree eq ==> flip impl) 
+                                                           (paco2 (@refines_ E1 E2 R1 R2 RE REAns RR) r).
 Admitted.
 
-Theorem refines_bind {E R1 R2 S1 S2} RR RS
-        (t1 : itree_spec E R1) (t2 : itree_spec E R2)
-        (k1 : R1 -> itree_spec E S1)
-        (k2 : R2 -> itree_spec E S2) :
-  refines RR t1 t2 -> (forall r1 r2, RR r1 r2 -> refines RS (k1 r1) (k2 r2)) ->
-  refines RS (ITree.bind t1 k1) (ITree.bind t2 k2).
+Theorem refines_bind {E1 E2 R1 R2 S1 S2} RE REAns RR RS
+        (t1 : itree_spec E1 R1) (t2 : itree_spec E2 R2)
+        (k1 : R1 -> itree_spec E1 S1)
+        (k2 : R2 -> itree_spec E2 S2) :
+  refines RE REAns RR t1 t2 -> (forall r1 r2, RR r1 r2 -> refines RE REAns RS (k1 r1) (k2 r2)) ->
+  refines RE REAns RS (ITree.bind t1 k1) (ITree.bind t2 k2).
 Proof.
   revert t1 t2. pcofix CIH.
   intros t1 t2 Ht12 Hk12. punfold Ht12. red in Ht12.
@@ -562,7 +575,13 @@ Proof.
   - rewrite Heqot1, Heqot2. repeat rewrite bind_tau. pstep. constructor.
     right. pclearbot. eapply CIH; eauto.
   - pclearbot. rewrite Heqot1, Heqot2. repeat rewrite bind_vis.
-    pstep. constructor. intros. right. eapply CIH; eauto. apply H.
+    pstep. constructor; auto. intros. right. eapply CIH; eauto. 
+
+    apply H0 in H1. pclearbot. auto.
+  - rewrite Heqot1, Heqot2. repeat rewrite bind_vis. pstep. constructor.
+    right. eapply CIH; eauto. pclearbot. apply H.
+  - rewrite Heqot1, Heqot2. repeat rewrite bind_vis. pstep. constructor.
+    right. eapply CIH; eauto. pclearbot. apply H.
   - rewrite Heqot2. rewrite bind_vis. pstep. constructor. intros.
     pstep_reverse.
   - rewrite Heqot1. rewrite bind_vis. pstep. econstructor. 
@@ -574,16 +593,17 @@ Qed.
 
 (*key lemma for iter here *)
 Lemma refines_iter_bind_aux:
-  forall (E : Type -> Type) (S2 S1 R1 R2 : Type) 
+  forall (E1 E2 : Type -> Type) (S2 S1 R1 R2 : Type) 
+    RE REAns
     (RR : R1 -> R2 -> Prop) (RS : S1 -> S2 -> Prop)
-    (k1 : R1 -> itree_spec E (R1 + S1))
-    (k2 : R2 -> itree_spec E (R2 + S2))
-    (r : itree_spec E S1 -> itree_spec E S2 -> Prop),
+    (k1 : R1 -> itree_spec E1 (R1 + S1))
+    (k2 : R2 -> itree_spec E2 (R2 + S2))
+    (r : itree_spec E1 S1 -> itree_spec E2 S2 -> Prop),
     (forall (r1 : R1) (r2 : R2),
         RR r1 r2 -> r (ITree.iter k1 r1) (ITree.iter k2 r2)) ->
-    forall (phi1 : itree_spec E (R1 + S1)) (phi2 : itree_spec E (R2 + S2)),
-      refines (HeterogeneousRelations.sum_rel RR RS) phi1 phi2 ->
-      paco2 (refines_ RS) r
+    forall (phi1 : itree_spec E1 (R1 + S1)) (phi2 : itree_spec E2 (R2 + S2)),
+      refines RE REAns (HeterogeneousRelations.sum_rel RR RS) phi1 phi2 ->
+      paco2 (refines_ RE REAns RS) r
             (phi1 >>=
                   (fun lr : R1 + S1 =>
                      match lr with
@@ -597,7 +617,7 @@ Lemma refines_iter_bind_aux:
                      | inr r0 => Ret r0
                      end)).
 Proof.
-  intros E S2 S1 R1 R2 RR RS k1 k2 r CIH.
+  intros E1 E2 S2 S1 R1 R2 RE REAns RR RS k1 k2 r CIH.
   pcofix CIH'. intros phi1 phi2 Hphi.
   punfold Hphi. red in Hphi.
   remember (observe phi1) as ophi1.
@@ -607,7 +627,12 @@ Proof.
     + pstep. constructor. right. eapply CIH; eauto.
     + pstep. constructor; auto.
   - setoid_rewrite bind_tau. pstep. constructor. right. eapply CIH'; eauto.
-  - setoid_rewrite bind_vis. pstep. constructor. right. eapply CIH'; eauto. apply H.
+  - setoid_rewrite bind_vis. pstep. constructor; auto. right. eapply CIH'; eauto. 
+    apply H0 in H1; pclearbot; eauto.
+  - repeat rewrite bind_vis. pstep. constructor. right. eapply CIH'; eauto.
+    apply H.
+  - repeat rewrite bind_vis. pstep. constructor. right. eapply CIH'; eauto.
+    apply H.
   - rewrite bind_vis. pstep. constructor. intros. pstep_reverse.
   - rewrite bind_vis. pstep. econstructor. pstep_reverse.
   - rewrite bind_vis. pstep. econstructor. pstep_reverse.
@@ -615,10 +640,10 @@ Proof.
 Qed.
 
 (*this one is going to be rougher going to require some nested coinduction, but should be manageable *)
-Theorem refines_iter {E R1 R2 S1 S2} (RR : R1 -> R2 -> Prop) (RS : S1 -> S2 -> Prop)
-        (k1 : R1 -> itree_spec E (R1 + S1)) (k2 : R2 -> itree_spec E (R2 + S2)) :
-  (forall r1 r2, RR r1 r2 -> refines (HeterogeneousRelations.sum_rel RR RS) (k1 r1) (k2 r2) ) ->
-  forall r1 r2, RR r1 r2 ->  refines RS (ITree.iter k1 r1) (ITree.iter k2 r2).
+Theorem refines_iter {E1 E2 R1 R2 S1 S2} RE REAns (RR : R1 -> R2 -> Prop) (RS : S1 -> S2 -> Prop)
+        (k1 : R1 -> itree_spec E1 (R1 + S1)) (k2 : R2 -> itree_spec E2 (R2 + S2)) :
+  (forall r1 r2, RR r1 r2 -> refines RE REAns (HeterogeneousRelations.sum_rel RR RS) (k1 r1) (k2 r2) ) ->
+  forall r1 r2, RR r1 r2 ->  refines RE REAns RS (ITree.iter k1 r1) (ITree.iter k2 r2).
 Proof.
   intros Hk. pcofix CIH. intros r1 r2 Hr12.
   rewrite unfold_iter. rewrite unfold_iter.
@@ -631,7 +656,11 @@ Proof.
     + pstep. constructor. auto.
   - setoid_rewrite bind_tau. pstep. constructor. left. pclearbot.
     eapply refines_iter_bind_aux; eauto.
-  - setoid_rewrite bind_vis. pstep. constructor. left. pclearbot.
+  - setoid_rewrite bind_vis. pstep. constructor; auto. left. pclearbot.
+    eapply refines_iter_bind_aux; eauto. apply H0 in H1; pclearbot; eauto.
+  - setoid_rewrite bind_vis. pstep. constructor; auto. left. pclearbot.
+    eapply refines_iter_bind_aux; eauto. apply H.
+  - setoid_rewrite bind_vis. pstep. constructor; auto. left. pclearbot.
     eapply refines_iter_bind_aux; eauto. apply H.
   - rewrite bind_vis. pstep. constructor. intros. pstep_reverse.
     eapply refines_iter_bind_aux; eauto; subst. all : pstep; apply H; auto.
